speedup

CollresMDfor1.0.ec
@@ -8,7 +8,7 @@ type msg.
 op uMsg: (msg * msg) distr.
 
 const IV: state.
- 
+
 const z0: block.
 
 (** f: ハッシュ関数 **)
@@ -19,7 +19,7 @@ op MD (m: msg) = fstar (pad m) IV.
 
 op coll(xy, xy': block * state) =
   xy <> xy' && f (fst xy) (snd xy) = f (fst xy') (snd xy').
- 
+
 axiom suffix_free:
   forall (m, m': msg, bl: block list), m <> m' => pad m <> bl ++ pad m'.
 
@@ -29,12 +29,8 @@ axiom fstar_nil:
 axiom fstar_cons:
   forall (x: block, y: state, xs: block list), fstar (x::xs) y = fstar xs (f x y).
 
-
 axiom size_behead : forall (xs: 'a list),
   0 < size xs => size(behead xs) < size xs.
-
-
-op head(xs : block list) = head z0 xs.
 
 module CR_MD = {
   proc oracle(m: msg) : state = {
@@ -50,7 +46,7 @@ module CR_MD = {
   proc main() : bool = {
     var m1, m2 : msg;
     var h1, h2 : state;
-    (m1, m2) <$ uMsg;
+    (m1, m2) = $uMsg;
     h1 <@ oracle(m1);
     h2 <@ oracle(m2);
     return (m1 <> m2 && h1 = h2);
@@ -58,6 +54,7 @@ module CR_MD = {
 }.
 
 module CR_f = {
+  var m1, m2: msg
   proc adv_b() : (block * state) * (block * state) = {
     var m1, m2 : msg;
     var y1, y2 : state;
@@ -67,7 +64,7 @@ module CR_f = {
     xs1 <- pad m1; y1 <- IV;
     xs2 <- pad m2; y2 <- IV;
     xs' <- [];
-    
+
     while (size xs2 < size xs1) {
       y1 <- f(head z0 xs1) y1;
       xs' <- xs' ++ [head z0 xs1];
@@ -93,81 +90,76 @@ module CR_f = {
 }.
 
 prover ["Alt-Ergo"].
-
-lemma MD_Collision_Resistance &m :
-    Pr[CR_MD.main() @ &m : res] <= Pr[CR_f.main() @ &m : res].
-    proof. byequiv=>//.
-    proc. 
-    inline CR_f.adv_b. seq 1 1 : (={m1, m2}). auto.
- 
-    seq 1 0 : ((h1 = MD m1){1} && ={m1, m2}). 
-    inline *; sp. wp.
+lemma MD_Collision_Resistance :
+equiv [CR_MD.main ~ CR_f.main : true ==> res{1} => res{2}].
+    proof.
+      proc. inline CR_f.adv_b. seq 1 1 : (={m1, m2}).
+      auto.
+      seq 1 0 : ((h1 = MD m1){1} && ={m1, m2}).
+      inline *; sp. wp.
     while{1} (fstar xs y = MD m1){1} (size xs{1}).
-    auto. smt(fstar_cons). 
-    skip. by progress; smt.
-    seq 1 0 : ((h1 = MD m1 && h2 = MD m2){1} && ={m1, m2}).
-    inline*. sp. wp.
-    while{1} (fstar xs y = MD m2){1} (size xs{1}). 
-    by auto; smt(fstar_cons). 
-    skip. by progress; smt. 
-sp.
-wp.
-(* m1 = m2 *)
-case (m1{2} = m2{2}).
-while{2} true (size xs1{2}). 
-progress. wp. skip. by progress; smt().
-rcondf{2} 1 => //.
-rcondf{2} 1 => //.
-skip. progress. smt.
+      auto => /> &m H xs_nonnil. split. rewrite - fstar_cons head_behead // size_behead. smt(fstar_cons).
+      skip => /> &2 xs y. split. move => ? ?; smt(size_ge0). rewrite fstar_nil =>//.
+      seq 1 0 : ((h1 = MD m1 && h2 = MD m2){1} && ={m1, m2}).
 
-(* m1 <> m2 /\ size xs1 <= size xs2 *)
-case (size xs1{2} <= size xs2{2}). 
-rcondf{2} 1. auto.  smt(size_behead).
-while{2} (fstar xs1 y1 = MD m1 &&
-    fstar xs2 y2 = MD m2 &&
-    (xs1 = xs2 => y1 <> y2) &&
-    size xs1 = size xs2){2} (size xs1){2}. 
-progress; auto; smt.
-while{2} (fstar xs2 y2 = MD m2 &&
-    xs' ++ xs2 = pad m2 &&
-    size xs1 <= size xs2){2}
-    (size xs2 - size xs1){2}. 
-by auto; progress; smt.
-skip; by progress; smt.
+      inline*; auto.
+    while{1} (fstar xs y = MD m2){1} (size xs{1}).
+    auto => /> &m ? ?. split. smt(fstar_cons). smt(size_ge0).
+    auto => /> &2 xs y. split. smt(size_ge0). rewrite fstar_nil => //.
 
-(* m1 <> m2 /\ size xs2 < size xs1 *)
+    sp. wp.
+      (* m1 = m2 *)
+    case (m1{2} = m2{2}).
+      while{2} true (size xs1{2}).
+    move => _ z. auto. move => &hr. smt(fstar_cons).
+    rcondf{2} 1 => //.
+    rcondf{2} 1 => //.
+    skip => /> xs1 xs2 y1 y2 ?. smt(size_ge0).
 
-  wp.
-  while{2} (fstar xs1 y1 = MD m1 && fstar xs2 y2 = MD m2 && size xs1 = size xs2 && (xs1 = xs2 => y1 <> y2)){2} (size xs1){2}. auto. smt.
-
-(* こちらの方法でも証明可能, ただしby smtによる外部ソルバ適用回数が増える
-while{2}  ((xs2{2} = pad m2{2} /\
-    y2{2} = IV /\
-    xs'{2} ++ xs1{2} = pad m1{2} /\
-    (h1{1} = MD m1{1} &&
-    h2{1} = MD m2{1}) && ={m1, m2}) /\
-    m1{2} <> m2{2} /\
-    size xs1{2} = size xs2{2} /\
-    (fstar xs1 y1 = MD m1)){2} (size xs2){2}. auto. progress; by smt.
-while{2} (fstar xs1 y1 = MD m1 && xs' ++ xs1 = pad m1 && size xs2 <= size xs1){2} (size xs1){2}. auto. progress; by smt.  
-skip. progress; by smt.
-*)
-
-seq{2} 0 1 : 
-    ((xs2{2} = pad m2{2} /\
-    y2{2} = IV /\
-    xs'{2} ++ xs1{2} = pad m1{2} /\
-    (h1{1} = MD m1{1} &&
-    h2{1} = MD m2{1}) && ={m1, m2}) /\
-    m1{2} <> m2{2} /\
-    size xs1{2} = size xs2{2} /\
-    (fstar xs1 y1 = MD m1){2}).
-while{2} (fstar xs1 y1 = MD m1 &&
-    xs' ++ xs1 = pad m1 &&
-    size xs2 <= size xs1){2}
+      (** m1 <> m2 /\ size xs1 <= size xs2 **)
+   case (size xs1{2} <= size xs2{2}).
+   rcondf{2} 1. auto => /> &hr ? ?. smt.
+    while{2} (
+      fstar xs1 y1 = MD m1 &&
+      fstar xs2 y2 = MD m2 &&
+      (xs1 = xs2 => y1 <> y2) &&
+      size xs1 = size xs2){2}
     (size xs1){2}.
-by auto; progress; smt.
-skip. progress; by smt.
-rcondf{2} 1. progress. skip. progress. smt.
-skip. by progress; smt.
+
+    auto => /> &hr ? ? ? ? ? ?. split. split. smt(fstar_cons). move => ?. split. rewrite - H0. rewrite - fstar_cons head_behead. smt. trivial.
+    move => ?. split. smt. move=>?. move:H2. smt. rewrite size_behead =>//. smt(size_ge0).
+
+    while{2} (fstar xs2 y2 = MD m2 &&
+      xs' ++ xs2 = pad m2 &&
+      size xs1 <= size xs2){2}
+    (size xs2 - size xs1){2}.
+
+    auto => /> ? ? ? ? ?. split. split. rewrite - fstar_cons. rewrite head_behead. smt. exact H.
+    move => ?. split. smt. move => ?. smt. rewrite StdOrder.IntOrder.ltr_le_sub. rewrite size_behead. smt. trivial.
+      skip; progress; by smt.
+      (* m1 <> m2 /\ size xs2 < size xs1 *)
+      wp.
+    while{2} (fstar xs1 y1 = MD m1 && fstar xs2 y2 = MD m2 && size xs1 = size xs2 && (xs1 = xs2 => y1 <> y2)){2} (size xs1){2}. auto => /> ? ? ? ? ? ? ?. split. split. rewrite - fstar_cons head_behead.
+      move: H4 =>//.
+      move: H1 =>//.
+    move => ?. split.
+      + rewrite - H0  - fstar_cons head_behead. smt.
+      trivial.
+    move => ?. split.
+      + smt.
+      + move => ? ?. smt.
+    rewrite size_behead. smt.
+
+      seq{2} 0 1 :
+    ((xs2{2} = pad m2{2} /\
+        y2{2} = IV /\
+      xs'{2} ++ xs1{2} = pad m1{2} /\ (h1{1} = MD m1{1} && h2{1} = MD m2{1}) && ={m1, m2}) /\
+      m1{2} <> m2{2} /\ size xs1{2} = size xs2{2} /\ (fstar xs1 y1 = MD m1){2}).
+
+     while{2} (fstar xs1 y1 = MD m1 && xs' ++ xs1 = pad m1 && size xs2 <= size xs1){2} (size xs1){2}.
+      progress. auto. progress; by smt.
+      skip. progress; by smt.
+
+      rcondf{2} 1; progress. skip. progress. smt.
+      skip. progress; by smt.
 qed.
